io/Compiler.MIO.To.Weak.fst
@@ -195,7 +195,7 @@ let make_rcs_eff (rcs:tree pck_rc) : typ_eff_rcs AllActions rcs =
   };
   r
 
-class exportable (styp : Type u#a) (pi:access_policy) (rcs:tree (pck_rc u#c u#d)) (fl:erased tflag) = {
+class exportable (styp : Type u#a) (pi:policy_spec) (rcs:tree (pck_rc u#c u#d)) (fl:erased tflag) = {
   [@@@no_method]
   wtyp : Type u#b;
   [@@@no_method]
@@ -204,7 +204,7 @@ class exportable (styp : Type u#a) (pi:access_policy) (rcs:tree (pck_rc u#c u#d)
   export : typ_eff_rcs fl rcs -> styp -> wtyp;
 }
 
-class safe_importable (styp : Type u#a) (pi:access_policy) (rcs:tree (pck_rc u#c u#d)) (fl:erased tflag) = {
+class safe_importable (styp : Type u#a) (pi:policy_spec) (rcs:tree (pck_rc u#c u#d)) (fl:erased tflag) = {
   [@@@no_method]
   swtyp : Type u#b;
   [@@@no_method]
@@ -213,7 +213,7 @@ class safe_importable (styp : Type u#a) (pi:access_policy) (rcs:tree (pck_rc u#c
   safe_import : swtyp -> typ_eff_rcs fl rcs -> styp; 
 }
 
-class importable (styp : Type u#a) (pi:access_policy) (rcs:tree (pck_rc u#c u#d)) (fl:erased tflag) = {
+class importable (styp : Type u#a) (pi:policy_spec) (rcs:tree (pck_rc u#c u#d)) (fl:erased tflag) = {
   [@@@no_method]
   wtyp : Type u#b; 
   [@@@no_method]
@@ -228,38 +228,38 @@ instance weak_safe_importable_super styp pi rcs fl (d : safe_importable styp pi 
 
 (** *** Exportable instances **)
 
-instance weak_is_exportable (#pi:access_policy) (#rcs:(tree pck_rc){Leaf? rcs}) (#fl:erased tflag) t {| d1: weak t fl pi |} : exportable t pi rcs fl = {
+instance weak_is_exportable (#pi:policy_spec) (#rcs:(tree pck_rc){Leaf? rcs}) (#fl:erased tflag) t {| d1: weak t fl pi |} : exportable t pi rcs fl = {
   wtyp = t;
   c_wtyp = solve;
   export = (fun Leaf x -> x)
 }
 
-instance exportable_unit (#pi:access_policy) (#fl:erased tflag) : exportable unit pi Leaf fl = {
+instance exportable_unit (#pi:policy_spec) (#fl:erased tflag) : exportable unit pi Leaf fl = {
   wtyp = unit;
   c_wtyp = solve;
   export = (fun Leaf () -> ())
 }
 
-instance exportable_file_descr (#pi:access_policy) (#fl:erased tflag) : exportable file_descr pi Leaf fl = {
+instance exportable_file_descr (#pi:policy_spec) (#fl:erased tflag) : exportable file_descr pi Leaf fl = {
   wtyp = file_descr;
   c_wtyp = solve;
   export = (fun Leaf fd -> fd)
 }
 
-instance exportable_bytes (#pi:access_policy) (#fl:erased tflag) : exportable Bytes.bytes pi Leaf fl = {
+instance exportable_bytes (#pi:policy_spec) (#fl:erased tflag) : exportable Bytes.bytes pi Leaf fl = {
   wtyp = Bytes.bytes;
   c_wtyp = solve;
   export = (fun Leaf b -> b)
 }
 
-instance exportable_refinement (#pi:access_policy) (#rcs:tree pck_rc) (#fl:erased tflag) t {| d:exportable t pi rcs fl |} (p : t -> Type0) : exportable (x:t{p x}) pi rcs fl = {
+instance exportable_refinement (#pi:policy_spec) (#rcs:tree pck_rc) (#fl:erased tflag) t {| d:exportable t pi rcs fl |} (p : t -> Type0) : exportable (x:t{p x}) pi rcs fl = {
   wtyp = d.wtyp;
   c_wtyp = solve;
   export = d.export
 }
 
 instance exportable_option
-  (#pi:access_policy) (#rcs:tree pck_rc) (#fl:erased tflag)
+  (#pi:policy_spec) (#rcs:tree pck_rc) (#fl:erased tflag)
   t1 {| d1:exportable t1 pi rcs fl |} :
   Tot (exportable (option t1) pi rcs fl) = {
   wtyp = option d1.wtyp;
@@ -269,7 +269,7 @@ instance exportable_option
 
 
 instance exportable_pair
-  (#pi:access_policy) (#rcs:(tree pck_rc){EmptyNode? rcs}) (#fl:erased tflag)
+  (#pi:policy_spec) (#rcs:(tree pck_rc){EmptyNode? rcs}) (#fl:erased tflag)
   t1 {| d1:exportable t1 pi (left rcs) fl |} t2 {| d2:exportable t2 pi (right rcs) fl |} :
   Tot (exportable (t1 * t2) pi rcs fl) = {
   wtyp = d1.wtyp * d2.wtyp;
@@ -278,7 +278,7 @@ instance exportable_pair
 }
 
 instance exportable_either
-  (#pi:access_policy) (#rcs:(tree pck_rc){EmptyNode? rcs}) (#fl:erased tflag)
+  (#pi:policy_spec) (#rcs:(tree pck_rc){EmptyNode? rcs}) (#fl:erased tflag)
   t1 {| d1:exportable t1 pi (left rcs) fl |} t2 {| d2:exportable t2 pi (right rcs) fl |} :
   Tot (exportable (either t1 t2) pi rcs fl) = {
   wtyp = either d1.wtyp d2.wtyp;
@@ -290,7 +290,7 @@ instance exportable_either
 (** *** Exportable arrows **)
 
 instance exportable_arrow_with_no_pre_and_no_post
-  (#pi:access_policy) (#rcs:(tree pck_rc){EmptyNode? rcs}) (#fl:erased tflag)
+  (#pi:policy_spec) (#rcs:(tree pck_rc){EmptyNode? rcs}) (#fl:erased tflag)
   (t1:Type) {| d1:importable t1 pi (left rcs) fl |}
   (t2:Type) {| d2:exportable t2 pi (right rcs) fl |} :
   exportable (t1 -> MIOpi (resexn t2) fl pi) pi rcs fl = {
@@ -309,7 +309,7 @@ instance exportable_arrow_with_no_pre_and_no_post
 
 (** This is a design choice for making proofs easier. One can remove the post-condition **)
 instance exportable_arrow_post_args
-  (#pi:access_policy) (#rcs:(tree pck_rc){EmptyNode? rcs}) (#fl:erased tflag)
+  (#pi:policy_spec) (#rcs:(tree pck_rc){EmptyNode? rcs}) (#fl:erased tflag)
   t1 {| d1:importable t1 pi (left rcs) fl |}
   t2 {| d2:exportable t2 pi (right rcs) fl |}
   (post : t1 -> trace -> resexn t2 -> trace -> Type0) 
@@ -323,7 +323,7 @@ instance exportable_arrow_post_args
   }
 
 instance exportable_arrow_post
-  (#pi:access_policy) (#rcs:(tree pck_rc){EmptyNode? rcs}) (#fl:erased tflag)
+  (#pi:policy_spec) (#rcs:(tree pck_rc){EmptyNode? rcs}) (#fl:erased tflag)
   t1 {| d1:importable t1 pi (left rcs) fl |}
   t2 {| d2:exportable t2 pi (right rcs) fl |}
   (post : trace -> resexn t2 -> trace -> Type0) 
@@ -377,7 +377,7 @@ let rwtyp_eff_rc #fl #a #b #c #d #rc eff_rc (x:c) =
 
 instance exportable_arrow_pre_post_args
   (t1:Type) (t2:Type)
-  (#pi:access_policy) 
+  (#pi:policy_spec) 
   (#rcs:(tree pck_rc){Node? rcs /\ arg_typ (root rcs) == t1 /\ (ret_typ (root rcs) == unit)})
   (#fl:erased tflag)
   {| d1:importable t1 pi (left rcs) fl |}
@@ -404,7 +404,7 @@ instance exportable_arrow_pre_post_args
 
 instance exportable_arrow_pre_post
   (t1:Type) (t2:Type)
-  (#pi:access_policy) 
+  (#pi:policy_spec) 
   (#rcs:(tree pck_rc){Node? rcs /\ arg_typ (root rcs) == unit /\ (ret_typ (root rcs) == unit)})
   (#fl:erased tflag)
   {| d1:importable t1 pi (left rcs) fl |}
@@ -431,25 +431,25 @@ instance exportable_arrow_pre_post
 
     
 (** *** Safe importable instances **)
-let weak_is_safely_importable (#pi:access_policy) (#rcs:(tree pck_rc){Leaf? rcs}) (#fl:erased tflag) #t (d:weak t fl pi) : safe_importable t pi rcs fl = {
+let weak_is_safely_importable (#pi:policy_spec) (#rcs:(tree pck_rc){Leaf? rcs}) (#fl:erased tflag) #t (d:weak t fl pi) : safe_importable t pi rcs fl = {
   swtyp = t;
   c_swtyp = solve;
   safe_import = (fun x Leaf -> x); 
 }
 
-instance importable_unit (#pi:access_policy) (#fl:erased tflag) : importable unit pi Leaf fl = {
+instance importable_unit (#pi:policy_spec) (#fl:erased tflag) : importable unit pi Leaf fl = {
   wtyp = unit;
   c_wtyp = solve;
   import = (fun () Leaf -> Inl ())
 }
 
-instance importable_file_descr (#pi:access_policy) (#fl:erased tflag) : importable file_descr pi Leaf fl = {
+instance importable_file_descr (#pi:policy_spec) (#fl:erased tflag) : importable file_descr pi Leaf fl = {
   wtyp = file_descr;
   c_wtyp = solve;
   import = (fun fd Leaf -> Inl fd)
 }
 
-instance importable_bytes (#pi:access_policy) (#fl:erased tflag) : importable Bytes.bytes pi Leaf fl = {
+instance importable_bytes (#pi:policy_spec) (#fl:erased tflag) : importable Bytes.bytes pi Leaf fl = {
   wtyp = Bytes.bytes;
   c_wtyp = solve;
   import = (fun b Leaf -> Inl b)
@@ -457,14 +457,14 @@ instance importable_bytes (#pi:access_policy) (#fl:erased tflag) : importable By
 
 (** *** Importable instances **)
 
-instance safe_importable_is_importable (#pi:access_policy) (#rcs:tree pck_rc) (#fl:erased tflag) #t (d:safe_importable t pi rcs fl) : importable t pi rcs fl = {
+instance safe_importable_is_importable (#pi:policy_spec) (#rcs:tree pck_rc) (#fl:erased tflag) #t (d:safe_importable t pi rcs fl) : importable t pi rcs fl = {
   wtyp = d.swtyp;
   c_wtyp = solve;
   import = (fun x eff_rcs -> Inl (d.safe_import x eff_rcs))
 }
 
 instance importable_refinement
-  (#pi:access_policy) (#rcs:tree pck_rc) (#fl:erased tflag)
+  (#pi:policy_spec) (#rcs:tree pck_rc) (#fl:erased tflag)
   t {| d:importable t pi rcs fl |}
   (rp : t -> Type0) {| d1:checkable rp |} :
   Tot (importable (x:t{rp x}) pi rcs fl) = {
@@ -479,7 +479,7 @@ instance importable_refinement
 }
     
 instance importable_option
-  (#pi:access_policy) (#rcs:tree pck_rc) (#fl:erased tflag)
+  (#pi:policy_spec) (#rcs:tree pck_rc) (#fl:erased tflag)
   t {| d:importable t pi rcs fl |} :
   Tot (importable (option t) pi rcs fl) = {
   wtyp = option d.wtyp;
@@ -495,7 +495,7 @@ instance importable_option
 }
 
 instance importable_pair
-  (#pi:access_policy) (#rcs:(tree pck_rc){EmptyNode? rcs}) (#fl:erased tflag)
+  (#pi:policy_spec) (#rcs:(tree pck_rc){EmptyNode? rcs}) (#fl:erased tflag)
   t1 t2 {| d1:importable t1 pi (left rcs) fl |} {| d2:importable t2 pi (right rcs) fl |} :
   Tot (importable (t1 * t2) pi rcs fl) = {
   wtyp = d1.wtyp * d2.wtyp;
@@ -507,7 +507,7 @@ instance importable_pair
 }
 
 instance importable_either
-  (#pi:access_policy) (#rcs:(tree pck_rc){EmptyNode? rcs}) (#fl:erased tflag)
+  (#pi:policy_spec) (#rcs:(tree pck_rc){EmptyNode? rcs}) (#fl:erased tflag)
   t1 t2 {| d1:importable t1 pi (left rcs) fl |} {| d2:importable t2 pi (right rcs) fl |} :
   Tot (importable (either t1 t2) pi rcs fl) = {
   wtyp = either d1.wtyp d2.wtyp;
@@ -527,7 +527,7 @@ instance importable_either
 }
 
 instance importable_dpair_refined
-  (#pi:access_policy) (#rcs:(tree pck_rc){EmptyNode? rcs}) (#fl:erased tflag)
+  (#pi:policy_spec) (#rcs:(tree pck_rc){EmptyNode? rcs}) (#fl:erased tflag)
   t1 t2 (p:t1 -> t2 -> Type0)
   {| d1:importable t1 pi (left rcs) fl |} {| d2:importable t2 pi (right rcs) fl |}
   {| d3:checkable2 p |} :
@@ -543,7 +543,7 @@ instance importable_dpair_refined
 
 (** *** Safe importable arrows **)
 instance safe_importable_resexn
-  (#pi:access_policy) (#rcs:tree pck_rc) (#fl:erased tflag)
+  (#pi:policy_spec) (#rcs:tree pck_rc) (#fl:erased tflag)
   t1 {| d1:importable t1 pi rcs fl |} :
   Tot (safe_importable (resexn t1) pi rcs fl) = {
   swtyp = resexn d1.wtyp;
@@ -555,7 +555,7 @@ instance safe_importable_resexn
 }
     
 instance safe_importable_arrow
-  (#pi:access_policy) (#rcs:(tree pck_rc){EmptyNode? rcs}) (#fl:erased tflag)
+  (#pi:policy_spec) (#rcs:(tree pck_rc){EmptyNode? rcs}) (#fl:erased tflag)
   (t1:Type) {| d1:exportable t1 pi (left rcs) fl |}
   (t2:Type) {| d2:importable t2 pi (right rcs) fl |} : 
   safe_importable ((x:t1) -> MIOpi (resexn t2) fl pi) pi rcs fl = {
@@ -572,7 +572,7 @@ let enforce_post_args_res
   (#t1:Type u#a)
   (#t2:Type u#b)
   (#fl:erased tflag)
-  (pi:access_policy)
+  (pi:policy_spec)
   (pre:t1 -> trace -> Type0)
   (post:t1 -> trace -> resexn t2 -> trace -> Type0)
   (rc : rc_typ t1 (resexn t2))
@@ -593,7 +593,7 @@ let enforce_post_args
   (#t1:Type u#a)
   (#t2:Type u#b)
   (#fl:erased tflag)
-  (pi:access_policy)
+  (pi:policy_spec)
   (pre:t1 -> trace -> Type0)
   (post:t1 -> trace -> resexn t2 -> trace -> Type0)
   (rc : rc_typ t1 unit)
@@ -614,7 +614,7 @@ let enforce_post_res
   (#t1:Type u#a)
   (#t2:Type u#b)
   (#fl:erased tflag)
-  (pi:access_policy)
+  (pi:policy_spec)
   (pre:t1 -> trace -> Type0)
   (post:t1 -> trace -> resexn t2 -> trace -> Type0)
   (rc : rc_typ unit (resexn t2))
@@ -635,7 +635,7 @@ let enforce_post
   (#t1:Type u#a)
   (#t2:Type u#b)
   (#fl:erased tflag)
-  (pi:access_policy)
+  (pi:policy_spec)
   (pre:t1 -> trace -> Type0)
   (post:t1 -> trace -> resexn t2 -> trace -> Type0)
   (rc : rc_typ unit unit)
@@ -654,7 +654,7 @@ let enforce_post
 
 instance safe_importable_arrow_pre_post_args_res
   (#t1:Type) (#t2:Type)
-  (#pi:access_policy) 
+  (#pi:policy_spec) 
   (#rcs:(tree pck_rc){Node? rcs /\ (arg_typ (root rcs) == t1 /\ (ret_typ (root rcs) == (resexn t2))) })
   (#fl:erased tflag)
   (pre : t1 -> trace -> Type0)
@@ -676,7 +676,7 @@ instance safe_importable_arrow_pre_post_args_res
 
 instance safe_importable_arrow_pre_post_res
   (#t1:Type) (#t2:Type)
-  (#pi:access_policy) 
+  (#pi:policy_spec) 
   (#rcs:(tree pck_rc){Node? rcs /\ (arg_typ (root rcs) == unit /\ (ret_typ (root rcs) == (resexn t2))) })
   (#fl:erased tflag)
   (pre : t1 -> trace -> Type0)
@@ -698,7 +698,7 @@ instance safe_importable_arrow_pre_post_res
 
 instance safe_importable_arrow_pre_post_args
   (#t1:Type) (#t2:Type)
-  (#pi:access_policy) 
+  (#pi:policy_spec) 
   (#rcs:(tree pck_rc){Node? rcs /\ (arg_typ (root rcs) == t1 /\ (ret_typ (root rcs) == unit)) })
   (#fl:erased tflag)
   (pre : t1 -> trace -> Type0)
@@ -723,7 +723,7 @@ instance safe_importable_arrow_pre_post
   (pre : t1 -> trace -> Type0)
   (post : t1 -> trace -> resexn t2 -> trace -> Type0)
 
-  (#pi:access_policy) 
+  (#pi:policy_spec) 
   (#rcs:(tree pck_rc){Node? rcs /\ (arg_typ (root rcs) == unit /\ (ret_typ (root rcs) == unit)) })
 
   (c1post : squash (forall x h lt. pre x h /\ enforced_locally pi h lt ==> post x h (Inr Contract_failure) lt))
